Logic/Logic/Kripke/Basic.lean
@@ -1,0 +1,224 @@
+import Logic.Logic.Semantics
+import Logic.Logic.System
+import Logic.Vorspiel.BinaryRelations
+
+universe u v
+-- set_option autoImplicit false
+
+namespace LO.Kripke
+
+structure Frame where
+  World : Type u
+  Rel : Rel World World
+  [World_nonempty : Nonempty World]
+
+instance : CoeSort Frame (Type u) := ⟨Frame.World⟩
+instance : CoeFun Frame (λ F => F.World → F.World → Prop) := ⟨Frame.Rel⟩
+
+instance {F : Frame} : Nonempty F.World := F.World_nonempty
+
+abbrev Frame.Rel' {F : Frame} (x y : F.World) := F.Rel x y
+scoped infix:45 " ≺ " => Frame.Rel'
+
+noncomputable abbrev Frame.default {F : Frame} : F.World := Classical.choice F.World_nonempty
+notation "﹫" => Frame.default
+
+
+set_option linter.unusedVariables false in
+abbrev Frame.Dep (α : Type v) := Frame.{u}
+
+abbrev Frame.alt (F : Frame.{u}) (α : Type v) : Frame.Dep α := F
+notation F:max "#" α:max => Frame.alt F α
+
+
+structure FiniteFrame extends Frame where
+  [World_finite : Finite World]
+
+instance {F : FiniteFrame} : Finite (F.World) := F.World_finite
+instance : Coe (FiniteFrame) (Frame) := ⟨λ F ↦ F.toFrame⟩
+
+
+open Relation (ReflTransGen TransGen)
+
+
+abbrev Frame.RelReflTransGen {F : Frame} : _root_.Rel F.World F.World:= ReflTransGen (· ≺ ·)
+scoped infix:45 " ≺^* " => Frame.RelReflTransGen
+
+namespace Frame.RelReflTransGen
+
+variable {F : Frame}
+
+@[simp] lemma single {x y : F.World} (hxy : x ≺ y) : x ≺^* y := ReflTransGen.single hxy
+
+@[simp] lemma reflexive : Reflexive F.RelReflTransGen := Relation.reflexive_reflTransGen
+
+@[simp] lemma refl {x : F.World} : x ≺^* x := reflexive x
+
+@[simp] lemma transitive : Transitive F.RelReflTransGen := Relation.transitive_reflTransGen
+
+@[simp] lemma symmetric : Symmetric F.Rel → Symmetric F.RelReflTransGen := ReflTransGen.symmetric
+
+end Frame.RelReflTransGen
+
+
+abbrev Frame.TransitiveReflexiveClosure (F : Frame) : Frame where
+  World := F.World
+  Rel := (· ≺^* ·)
+postfix:max "^*" => Frame.TransitiveReflexiveClosure
+
+namespace Frame.TransitiveReflexiveClosure
+
+variable {F : Frame}
+
+lemma single {x y : F.World} (hxy : x ≺ y) : F^*.Rel x y := ReflTransGen.single hxy
+
+lemma rel_reflexive : Reflexive F^*.Rel := by intro x; exact ReflTransGen.refl;
+
+lemma rel_transitive : Transitive F^*.Rel := by simp;
+
+lemma rel_symmetric : Symmetric F.Rel → Symmetric F^* := ReflTransGen.symmetric
+
+end Frame.TransitiveReflexiveClosure
+
+
+
+abbrev Frame.RelTransGen {F : Frame} : _root_.Rel F.World F.World := TransGen (· ≺ ·)
+scoped infix:45 " ≺^+ " => Frame.RelTransGen
+
+namespace Frame.RelTransGen
+
+variable {F : Frame}
+
+@[simp] lemma single {x y : F.World} (hxy : x ≺ y) : x ≺^+ y := TransGen.single hxy
+
+@[simp]
+lemma transitive : Transitive F.RelTransGen := λ _ _ _ => TransGen.trans
+
+@[simp]
+lemma symmetric (hSymm : Symmetric F.Rel) : Symmetric F.RelTransGen := by
+  intro x y rxy;
+  induction rxy with
+  | single h => exact TransGen.single $ hSymm h;
+  | tail _ hyz ih => exact TransGen.trans (TransGen.single $ hSymm hyz) ih
+
+end Frame.RelTransGen
+
+
+abbrev Frame.TransitiveClosure (F : Frame) : Frame where
+  World := F.World
+  Rel := (· ≺^+ ·)
+scoped postfix:max "^+" => Frame.TransitiveClosure
+
+namespace Frame.TransitiveClosure
+
+variable {F : Frame}
+
+lemma single {x y : F.World} (hxy : x ≺ y) : F^+ x y := TransGen.single hxy
+
+lemma rel_transitive : Transitive F^+ := by simp;
+
+lemma rel_symmetric (hSymm : Symmetric F.Rel) : Symmetric F.TransitiveClosure := by simp_all
+
+end Frame.TransitiveClosure
+
+
+abbrev FrameClass := Set (Frame)
+
+set_option linter.unusedVariables false in
+abbrev FrameClass.Dep (α : Type v) := FrameClass.{u}
+
+abbrev FrameClass.alt (𝔽 : FrameClass) (α) : FrameClass.Dep α := 𝔽
+notation 𝔽:max "#" α:max => FrameClass.alt 𝔽 α
+
+/-
+abbrev FiniteFrameClass := Set (FiniteFrame)
+
+@[simp] def FiniteFrameClass.toFrameClass (𝔽 : FiniteFrameClass) : FrameClass := { F | ∃ F', F' ∈ 𝔽 ∧ F'.toFrame = F }
+instance : Coe (FiniteFrameClass) (FrameClass) := ⟨FiniteFrameClass.toFrameClass⟩
+
+@[simp] def FrameClass.toFiniteFrameClass (𝔽 : FrameClass) : FiniteFrameClass := { F | F.toFrame ∈ 𝔽 }
+instance : Coe (FrameClass) (FiniteFrameClass) := ⟨FrameClass.toFiniteFrameClass⟩
+
+@[simp] abbrev FrameClass.restrictFinite (𝔽 : FrameClass) : FrameClass := FiniteFrameClass.toFrameClass ↑𝔽
+postfix:max "ꟳ" => FrameClass.restrictFinite
+
+lemma FrameClass.iff_mem_restrictFinite {𝔽 : FrameClass} {F : Frame} (h : F ∈ 𝔽) (F_finite : Finite F.World) : F ∈ 𝔽ꟳ := by
+  simp;
+  use { toFrame := F, World_finite := F_finite };
+-/
+
+-- set_option pp.universes true in
+/-
+abbrev FrameClassOfSystem {F : Type u} [System F S] (𝓢 : S) (α : Type u) [Semantics F (Frame.Dep α)] : FrameClass.Dep α := { F | F ⊧* System.theory 𝓢 }
+notation "𝔽(" 𝓢 " of " α ")" => FrameClassOfSystem 𝓢 α
+-/
+
+section
+
+/-- FrameClass for `𝐈𝐧𝐭` and `𝐒𝟒` -/
+abbrev ReflexiveTransitiveFrameClass : FrameClass := λ F => Reflexive F ∧ Transitive F
+
+/-- FrameClass for `𝐊𝐂` and `𝐒𝟒.𝟐` -/
+abbrev ReflexiveTransitiveConfluentFrameClass : FrameClass := λ F => Reflexive F ∧ Transitive F ∧ Confluent F
+
+/-- FrameClass for `𝐋𝐂` and `𝐒𝟒.𝟑` -/
+abbrev ReflexiveTransitiveConnectedFrameClass : FrameClass := λ F => Reflexive F ∧ Transitive F ∧ Connected F
+
+/-- FrameClass for `𝐂𝐥` and `𝐊𝐓𝟒𝐁` (`𝐒𝟓`) -/
+abbrev ReflexiveTransitiveSymmetricFrameClass : FrameClass := λ F => Reflexive F ∧ Transitive F ∧ Symmetric F
+
+end
+
+/-- `𝔽₁` is characterized by `𝔽₂` -/
+class FrameClass.Characteraizable (𝔽₁ : FrameClass) (𝔽₂ : outParam (FrameClass)) where
+  characterize : ∀ {F}, F ∈ 𝔽₂ → F ∈ 𝔽₁
+  nonempty : ∃ F, F ∈ 𝔽₂
+
+
+abbrev Valuation (F : Frame) (α : Type*) := F.World → α → Prop
+
+abbrev Valuation.atomic_hereditary (V : Valuation F α) : Prop := ∀ {w₁ w₂ : F.World}, (w₁ ≺ w₂) → ∀ {a}, (V w₁ a) → (V w₂ a)
+
+
+structure Model (α) where
+  Frame : Frame
+  Valuation : Valuation Frame α
+
+abbrev Model.World (M : Model α) := M.Frame.World
+instance : CoeSort (Model α) (Type u) := ⟨Model.World⟩
+
+
+section Classical
+
+abbrev ClassicalFrame : Kripke.Frame where
+  World := Unit
+  Rel _ _ := True
+
+
+namespace ClassicalFrame
+
+@[simp] lemma transitive : Transitive ClassicalFrame := by simp [Transitive];
+
+@[simp] lemma reflexive : Reflexive ClassicalFrame := by simp [Reflexive];
+
+@[simp] lemma euclidean : Euclidean ClassicalFrame := by simp [Euclidean];
+
+@[simp] lemma symmetric : Symmetric ClassicalFrame := by simp [Symmetric];
+
+@[simp] lemma extensive : Extensive ClassicalFrame := by simp [Extensive];
+
+@[simp] lemma universal : Universal ClassicalFrame := by simp [Universal];
+
+end ClassicalFrame
+
+
+abbrev ClassicalValuation (α : Type*) := α → Prop
+
+abbrev ClassicalModel (V : ClassicalValuation α) : Kripke.Model α where
+  Frame := ClassicalFrame
+  Valuation _ a := V a
+
+end Classical
+
+
+end LO.Kripke
